attempt to cleanup defs

compiler/backend/backend_passesScript.sml
@@ -180,19 +180,10 @@ Proof
           bvi_to_dataTheory.compile_exp_def,bvi_to_dataTheory.optimise_def]
 QED
 
-Definition to_word_all_def:
-  to_word_all (c:'a config) p =
-    let (ps,c,p,names) = to_data_all c p in
-    let data_conf = c.data_conf in
+Definition word_internal_def:
+  word_internal ps (c:'a config) names p =
     let word_conf = c.word_to_word_conf in
     let asm_conf = c.lab_conf.asm_conf in
-    let data_conf =
-            data_conf with
-            <|has_fp_ops := (1 < asm_conf.fp_reg_count);
-              has_fp_tern :=
-                (asm_conf.ISA = ARMv7 ∧ 2 < asm_conf.fp_reg_count)|> in
-    let p = stubs (:α) data_conf ++ MAP (compile_part data_conf) p in
-    let ps = ps ++ [(strlit "after data_to_word",Word p names)] in
     let (two_reg_arith,reg_count) =
             (asm_conf.two_reg_arith,
              asm_conf.reg_count − (5 + LENGTH asm_conf.avoid_regs)) in
@@ -210,6 +201,9 @@ Definition to_word_all_def:
                   ((name_num,arg_count,full_ssa_cc_trans arg_count prog),col_opt)) p in
     let ps = ps ++ [(strlit "after word_ssa",Word (MAP FST p) names)] in
     let p = MAP (λ((name_num,arg_count,prog),col_opt).
+                  ((name_num,arg_count,remove_dead_prog prog),col_opt)) p in
+    let ps = ps ++ [(strlit "after remove_dead in word_ssa",Word (MAP FST p) names)] in
+    let p = MAP (λ((name_num,arg_count,prog),col_opt).
                   ((name_num,arg_count,word_common_subexp_elim prog),col_opt)) p in
     let ps = ps ++ [(strlit "after word_cse",Word (MAP FST p) names)] in
     let p = MAP (λ((name_num,arg_count,prog),col_opt).
@@ -217,13 +211,13 @@ Definition to_word_all_def:
     let ps = ps ++ [(strlit "after word_copy",Word (MAP FST p) names)] in
     let p = MAP (λ((name_num,arg_count,prog),col_opt).
                   ((name_num,arg_count,
-                   if two_reg_arith then three_to_two_reg prog else prog),col_opt)) p in
+                   three_to_two_reg_prog two_reg_arith prog),col_opt)) p in
     let ps = ps ++ [(strlit "after three_to_two_reg from word_inst",Word (MAP FST p) names)] in
     let p = MAP (λ((name_num,arg_count,prog),col_opt).
                   ((name_num,arg_count,remove_unreach prog),col_opt)) p in
     let ps = ps ++ [(strlit "after word_unreach",Word (MAP FST p) names)] in
     let p = MAP (λ((name_num,arg_count,prog),col_opt).
-                  ((name_num,arg_count,FST (remove_dead prog LN)),col_opt)) p in
+                  ((name_num,arg_count,remove_dead_prog prog)),col_opt) p in
     let ps = ps ++ [(strlit "after remove_dead in word_alloc",Word (MAP FST p) names)] in
     let p = MAP (λ((name_num,arg_count,prog),col_opt).
                   ((name_num,arg_count,
@@ -231,6 +225,22 @@ Definition to_word_all_def:
                      (word_alloc name_num asm_conf alg reg_count prog col_opt)))) p in
     let ps = ps ++ [(strlit "after word_alloc (and remove_must_terminate)",Word p names)] in
     let c = c with word_to_word_conf updated_by (λc. c with col_oracle := col) in
+    (p,ps,c)
+End
+
+Definition to_word_all_def:
+  to_word_all (c:'a config) p =
+    let (ps,c,p,names) = to_data_all c p in
+    let data_conf = c.data_conf in
+    let asm_conf = c.lab_conf.asm_conf in
+    let data_conf =
+            data_conf with
+            <|has_fp_ops := (1 < asm_conf.fp_reg_count);
+              has_fp_tern :=
+                (asm_conf.ISA = ARMv7 ∧ 2 < asm_conf.fp_reg_count)|> in
+    let p = stubs (:α) data_conf ++ MAP (compile_part data_conf) p in
+    let ps = ps ++ [(strlit "after data_to_word",Word p names)] in
+    let (p,ps,c) = word_internal ps c names p in
       ((ps: (mlstring # 'a any_prog) list),c,p,names)
 End
 
@@ -238,7 +248,8 @@ Theorem to_word_thm:
   SND (to_word_all (c:'a config) p) = to_word c p
 Proof
   assume_tac to_data_thm
-  \\ fs [to_word_all_def,to_word_def,data_to_wordTheory.compile_def,
+  \\ fs [to_word_all_def,word_internal_def,
+         to_word_def,data_to_wordTheory.compile_def,
          word_to_wordTheory.compile_def]
   \\ rpt (pairarg_tac \\ gvs [])
   \\ gvs [MAP_MAP_o,o_DEF,LAMBDA_PROD]
@@ -369,53 +380,14 @@ QED
 
 Definition from_word_0_all_def:
   from_word_0_all ps (c:'a config) names p =
-    let word_conf = c.word_to_word_conf in
-    let asm_conf = c.lab_conf.asm_conf in
-    let (two_reg_arith,reg_count) =
-            (asm_conf.two_reg_arith,
-             asm_conf.reg_count − (5 + LENGTH asm_conf.avoid_regs)) in
-    let (n_oracles,col) = next_n_oracle (LENGTH p) word_conf.col_oracle in
-    let p = ZIP (p,n_oracles) in
-    let alg = word_conf.reg_alg in
-    let p = MAP (λ((name_num,arg_count,prog),col_opt).
-                  ((name_num,arg_count,word_simp$compile_exp prog),col_opt)) p in
-    let ps = ps ++ [(strlit "after word_simp",Word (MAP FST p) names)] in
-    let p = MAP (λ((name_num,arg_count,prog),col_opt).
-                  ((name_num,arg_count,
-                     inst_select asm_conf (max_var prog + 1) prog),col_opt)) p in
-    let ps = ps ++ [(strlit "after word_inst",Word (MAP FST p) names)] in
-    let p = MAP (λ((name_num,arg_count,prog),col_opt).
-                  ((name_num,arg_count,full_ssa_cc_trans arg_count prog),col_opt)) p in
-    let ps = ps ++ [(strlit "after word_ssa",Word (MAP FST p) names)] in
-    let p = MAP (λ((name_num,arg_count,prog),col_opt).
-                  ((name_num,arg_count,word_common_subexp_elim prog),col_opt)) p in
-    let ps = ps ++ [(strlit "after word_cse",Word (MAP FST p) names)] in
-    let p = MAP (λ((name_num,arg_count,prog),col_opt).
-                  ((name_num,arg_count,copy_prop prog),col_opt)) p in
-    let ps = ps ++ [(strlit "after word_copy",Word (MAP FST p) names)] in
-    let p = MAP (λ((name_num,arg_count,prog),col_opt).
-                  ((name_num,arg_count,
-                   if two_reg_arith then three_to_two_reg prog else prog),col_opt)) p in
-    let ps = ps ++ [(strlit "after three_to_two_reg from word_inst",Word (MAP FST p) names)] in
-    let p = MAP (λ((name_num,arg_count,prog),col_opt).
-                  ((name_num,arg_count,remove_unreach prog),col_opt)) p in
-    let ps = ps ++ [(strlit "after word_unreach",Word (MAP FST p) names)] in
-    let p = MAP (λ((name_num,arg_count,prog),col_opt).
-                  ((name_num,arg_count,FST (remove_dead prog LN)),col_opt)) p in
-    let ps = ps ++ [(strlit "after remove_dead in word_alloc",Word (MAP FST p) names)] in
-    let p = MAP (λ((name_num,arg_count,prog),col_opt).
-                  ((name_num,arg_count,
-                   remove_must_terminate
-                     (word_alloc name_num asm_conf alg reg_count prog col_opt)))) p in
-    let ps = ps ++ [(strlit "after word_alloc (and remove_must_terminate)",Word p names)] in
-    let c = c with word_to_word_conf updated_by (λc. c with col_oracle := col) in
+    let (p,ps,c) = word_internal ps c names p in
       from_word_all ps c names p
 End
 
 Theorem from_word_0_thm:
   SND (from_word_0_all ps c names p) = from_word_0 c names p
 Proof
-  gvs [from_word_0_all_def,from_word_0_def]
+  gvs [from_word_0_all_def,word_internal_def,from_word_0_def]
   \\ fs [to_word_all_def,to_word_def,data_to_wordTheory.compile_def,
          word_to_wordTheory.compile_def]
   \\ rpt (pairarg_tac \\ gvs [])
@@ -469,12 +441,12 @@ Proof
 QED
 
 Theorem number_of_passes:
-  LENGTH (FST (to_target_all c p)) = 38
+  LENGTH (FST (to_target_all c p)) = 39
 Proof
   fs [to_target_all_def] \\ rpt (pairarg_tac \\ gvs [])
   \\ fs [to_lab_all_def] \\ rpt (pairarg_tac \\ gvs [])
   \\ fs [to_stack_all_def] \\ rpt (pairarg_tac \\ gvs [])
-  \\ fs [to_word_all_def] \\ rpt (pairarg_tac \\ gvs [])
+  \\ fs [word_internal_def,to_word_all_def] \\ rpt (pairarg_tac \\ gvs [])
   \\ fs [to_data_all_def] \\ rpt (pairarg_tac \\ gvs [])
   \\ fs [to_bvi_all_def] \\ rpt (pairarg_tac \\ gvs [])
   \\ fs [to_bvl_all_def] \\ rpt (pairarg_tac \\ gvs [])
