compiler/backend/backendScript.sml
@@ -326,12 +326,12 @@ Definition to_livesets_def:
     let maxv = max_var prog + 1 in
     let inst_prog = inst_select asm_conf maxv prog in
     let ssa_prog = full_ssa_cc_trans arg_count inst_prog in
-    let cse_prog = word_common_subexp_elim ssa_prog in
+    let rm_ssa_prog = remove_dead_prog ssa_prog in
+    let cse_prog = word_common_subexp_elim rm_ssa_prog in
     let cp_prog = copy_prop cse_prog in
-    let two_prog = if two_reg_arith then three_to_two_reg cp_prog
-                                else cp_prog in
+    let two_prog = three_to_two_reg_prog two_reg_arith cp_prog in
     let unreach_prog = remove_unreach two_prog in
-    let rm_prog = FST(remove_dead unreach_prog LN) in
+    let rm_prog = remove_dead_prog unreach_prog in
      (name_num,arg_count,rm_prog)) p in
   let data = MAP (\(name_num,arg_count,prog).
     let (heu_moves,spillcosts) = get_heuristics alg name_num prog in
@@ -351,12 +351,12 @@ Definition to_livesets_0_def:
     let maxv = max_var prog + 1 in
     let inst_prog = inst_select asm_conf maxv prog in
     let ssa_prog = full_ssa_cc_trans arg_count inst_prog in
-    let cse_prog = word_common_subexp_elim ssa_prog in
+    let rm_ssa_prog = remove_dead_prog ssa_prog in
+    let cse_prog = word_common_subexp_elim rm_ssa_prog in
     let cp_prog = copy_prop cse_prog in
-    let two_prog = if two_reg_arith then three_to_two_reg cp_prog
-                                else cp_prog in
+    let two_prog = three_to_two_reg_prog two_reg_arith cp_prog in
     let unreach_prog = remove_unreach two_prog in
-    let rm_prog = FST(remove_dead unreach_prog LN) in
+    let rm_prog = remove_dead_prog unreach_prog in
      (name_num,arg_count,rm_prog)) p in
   let data = MAP (\(name_num,arg_count,prog).
     let (heu_moves,spillcosts) = get_heuristics alg name_num prog in
